refactor Logic/Function refactor Meta/Function

GMLInit/Logic/Function.lean
@@ -2,40 +2,59 @@ import GMLInit.Logic.Basic
 
 namespace Function
 
-abbrev curry {α β γ} (f : α × β → γ) (a : α) (b : β) := f (a,b)
+abbrev curry {α} {β : α → Sort _} {γ : (a : α) ×' β a → Sort _} (f : (p : (a : α) ×' β a) → γ p) (a : α) (b : β a) : γ ⟨a, b⟩ := f ⟨a, b⟩
 
-abbrev uncurry {α β γ} (f : α → β → γ) (ab : α × β) := f ab.fst ab.snd
+abbrev uncurry {α} {β : α → Sort _} {γ : {a : α} → β a → Sort _} (f : (a : α) → (b : β a) → γ b) (ab : (a : α) ×' β a) : γ ab.snd := f ab.fst ab.snd
 
-abbrev dcurry {α} {β : α → Sort _} {γ : (a : α) × β a → Sort _} (f : (p : (a : α) × β a) → γ p) (a : α) (b : β a) : γ ⟨a, b⟩ := f ⟨a, b⟩
+syntax (name := curryNum) "curry." noWs num term : term
+macro_rules
+| `(curry.$n:num $f:term) =>
+  match n.isNatLit? with
+  | some 0 => `($f)
+  | some (n+1) =>
+    let n := Lean.Syntax.mkNumLit (toString n)
+    `(curry.$n (Function.curry $f))
+  | _ => Lean.Macro.throwUnsupported
 
-abbrev duncurry {α} {β : α → Sort _} {γ : {a : α} → β a → Sort _} (f : (a : α) → (b : β a) → γ b) (ab : (a : α) × β a) : γ ab.snd := f ab.fst ab.snd
+syntax (name := uncurryNum) "uncurry." noWs num term : term
+macro_rules
+| `(uncurry.$n:num $f:term) =>
+  match n.isNatLit? with
+  | some 0 => `($f)
+  | some (n+1) =>
+    let n := Lean.Syntax.mkNumLit (toString n)
+    `(uncurry.$n (Function.uncurry $f))
+  | _ => Lean.Macro.throwUnsupported
 
-class InjectiveT {α β} (f : α → β) : Prop where
-  protected inj {a₁ a₂} : f a₁ = f a₂ → a₁ = a₂
+class InjectiveTC {α β} (f : α → β) : Prop where
+  protected inj {lhs rhs} : f lhs = f rhs → lhs = rhs
 
-export InjectiveT (inj)
+class Injective {α β} (f : α → β) extends InjectiveTC f : Prop
 
-abbrev injection {α β} (f : α → β) [InjectiveT f] {lhs rhs : α} : f lhs = f rhs → lhs = rhs := inj
+def inj {α β} (f : α → β) [self : InjectiveTC f] {lhs rhs} : f lhs = f rhs → lhs = rhs := self.inj
 
-theorem injectionIff {α β} (f : α → β) [InjectiveT f] {a₁ a₂ : α} : f a₁ = f a₂ ↔ a₁ = a₂ := Iff.intro inj (congrArg f)
+theorem inj_iff {α β} (f : α → β) [InjectiveTC f] {lhs rhs : α} : f lhs = f rhs ↔ lhs = rhs := Iff.intro (inj f) (congrArg f)
 
-theorem injectionEq {α β} (f : α → β) [InjectiveT f] {a₁ a₂ : α} : (f a₁ = f a₂) = (a₁ = a₂) := propext (injectionIff f)
+theorem inj_eq {α β} (f : α → β) [InjectiveTC f] {lhs rhs : α} : (f lhs = f rhs) = (lhs = rhs) := propext (inj_iff f)
 
-class Injective {α β} (f : α → β) extends InjectiveT f : Prop
+namespace Injective
 
-protected instance InjectiveT.comp {α β γ} (g : α → β) (f : β → γ) [Injective f] [InjectiveT g] : InjectiveT (f $ g .) where
-  inj {x₁ x₂} h := inj (inj h)
+instance {α β γ} (g : α → β) (f : β → γ) [Injective f] [InjectiveTC g] : InjectiveTC (λ x => f (g x)) where
+  inj h := inj g (inj f h)
 
 instance (α) : Injective (id : α → α) where inj := id
-instance (α β) : Injective (Sum.inl : α → Sum α β) where inj := Sum.inl.inj
-instance (α β) : Injective (Sum.inr : β → Sum α β) where inj := Sum.inr.inj
-instance (α β) (a : α) : Injective ((a,.) : β → α × β) where inj := λ h => (Prod.mk.inj h).right
-instance (α β) (b : β) : Injective ((.,b) : α → α × β) where inj := λ h => (Prod.mk.inj h).left
-instance (a : α) : Injective (a::.) where inj := λ h => (List.cons.inj h).2
-instance (as : List α) : Injective (.::as) where inj := λ h => (List.cons.inj h).left
-instance (α) : Injective (some : α → Option α) where inj := Option.some.inj
-instance : Injective Nat.succ where inj := Nat.succ.inj
+instance (α β) : Injective (Sum.inl : α → Sum α β) where inj | rfl => rfl
+instance (α β) : Injective (Sum.inr : β → Sum α β) where inj | rfl => rfl
+instance (α β) (b : β) : Injective ((.,b) : α → α × β) where inj | rfl => rfl
+instance (α β) (a : α) : Injective ((a,.) : β → α × β) where inj | rfl => rfl
+instance (α) (β : α → Type _) (a : α) : Injective (Sigma.mk a : β a → Sigma β) where inj | rfl => rfl
+instance (a : α) : Injective (a::.) where inj | rfl => rfl
+instance (as : List α) : Injective (.::as) where inj | rfl => rfl
+instance (α) : Injective (some : α → Option α) where inj | rfl => rfl
+instance : Injective Nat.succ where inj | rfl => rfl
 instance (n : Nat) : Injective (n+.: Nat → Nat) where inj := Nat.add_left_cancel
 instance (n : Nat) : Injective (.+n: Nat → Nat) where inj := Nat.add_right_cancel
+
+end Injective
 
 end Function
