GMLInit/Meta/Function.lean
@@ -2,14 +2,14 @@ import GMLInit.Meta.Basic
 import GMLInit.Logic.Function
 
 namespace Meta
-open Lean.Parser.Tactic
+open Lean.Parser.Tactic (location)
 
-syntax "injectivity" (term)? (location)? : tactic
+syntax "injectivity " (term:max)? (location)? : tactic
 
 macro_rules
-| `(tactic|injectivity $f) => `(tactic|apply Function.injection $f)
-| `(tactic|injectivity at $hs:ident*) => `(tactic|rw [Function.injectionEq] at $hs:ident*)
-| `(tactic|injectivity $f at $hs:ident*) => `(tactic|rw [Function.injectionEq $f] at $hs:ident*)
-| `(tactic|injectivity $f at $hs:ident* ⊢) => `(tactic|injectivity $f at $hs:ident*; injectivity $f)
+| `(tactic| injectivity $f) => `(tactic| apply Function.inj $f)
+| `(tactic| injectivity at $hs:ident*) => `(tactic| rw [Function.inj_eq] at $hs:ident*)
+| `(tactic| injectivity $f at $hs:ident*) => `(tactic| rw [Function.inj_eq $f] at $hs:ident*)
+| `(tactic| injectivity $f at $hs:ident* ⊢) => `(tactic| injectivity $f at $hs:ident*; injectivity $f)
 
 end Meta
